src/hmem/encoding/emulator.lean
@@ -33,6 +33,34 @@ begin
   exact rfl,
 end
 
+instance fin_memory_encoding {α: Type*} [fintype μ] [complexity.has_encoding (runtime_model μ) α]:
+  complexity.has_encoding (runtime_model μ) (μ → α) :=
+begin
+  fconstructor,
+  fconstructor,
+  exact λ f, quotient.mk (hidden.memory.node (0:μ) (λ u, memory.out (encode (f u)))),
+  intros x y,
+  split,
+  intro p,
+  funext u,
+  have h := congr_fun (congr_arg memory.getm p) u,
+  rw [memory.getm_mk, memory.getm_mk] at h,
+  unfold hidden.getm at h,
+  rw [memory.out_eq, memory.out_eq] at h,
+  apply encode_inj h,
+  intro h,
+  rw [h],
+  exact rfl,
+end
+
+-- def encode_vector_function {α: Type*} [complexity.has_encoding (runtime_model μ) α] [∀ {β: Type*} [complexity.has_encoding (runtime_model μ) β], complexity.has_encoding (runtime_model μ) (μ → β)]:
+--   Π (n: ℕ), (vector μ n → α) → memory μ
+-- | 0 f := encode (f vector.nil)
+-- | (n+1) f := encode (λ u, encode_vector_function 
+
+-- end
+
+
 -- def encode_instruction: instruction μ → memory μ
 -- | vop {n: ℕ} (op: vector α n → α) (dst: source α) (src: vector (source α) n): instruction
 -- | mop (op: hmem.instruction.memory_operation) (dst src: source α): instruction
